clean up userbase example

example_userbase.thy
@@ -14,7 +14,7 @@ begin
 
 
 datatype val =
-    String string
+  String string
   | UserId int
   | Bool bool
   | Undef
@@ -61,7 +61,7 @@ fun stringval where
 | "stringval _ = ''''"
 
 datatype userDataOp =
-    Name "val registerOp"
+  Name "val registerOp"
   | Mail "val registerOp"
 
 
@@ -89,6 +89,7 @@ type_synonym operation =
 
 
 
+text_raw \<open>\DefineSnippet{userbase_impl}{\<close>
 definition registerUser_impl :: "val \<Rightarrow> val \<Rightarrow> (val,operation,val) io" where
   "registerUser_impl name mail \<equiv>  do {
   u \<leftarrow> newId isUserId;
@@ -98,7 +99,6 @@ definition registerUser_impl :: "val \<Rightarrow> val \<Rightarrow> (val,operat
   });
   return u
 }"
-
 
 definition updateMail_impl :: "val \<Rightarrow> val \<Rightarrow> (val,operation,val) io" where
   "updateMail_impl u mail \<equiv>  do {
@@ -110,7 +110,6 @@ definition updateMail_impl :: "val \<Rightarrow> val \<Rightarrow> (val,operatio
   });
   return Undef
 }"
-
 
 definition removeUser_impl :: "val \<Rightarrow> (val,operation,val) io" where
   "removeUser_impl u \<equiv>  do {
@@ -131,6 +130,8 @@ definition getUser_impl :: "val \<Rightarrow> (val,operation,val) io" where
     } else return NotFound)
   })
 }"
+text_raw \<open>}%EndSnippet\<close>
+
 
 
 
@@ -176,6 +177,7 @@ definition procedures :: "proc \<Rightarrow> (localState \<times> (localState, o
   | GetUser u  \<Rightarrow>  toImpl' invoc (getUser_impl (UserId u))
 "
 
+text_raw \<open>\DefineSnippet{userbase_invariants}{\<close>
 definition inv1  where
   "inv1 op res ihb \<equiv> \<forall>r g u g_res.
     op r \<triangleq> RemoveUser u
@@ -185,48 +187,37 @@ definition inv1  where
   \<longrightarrow> g_res = NotFound"
 
 definition inv2  where
-  "inv2 op i_origin c_calls \<equiv> \<forall>u i c.
-    op i \<triangleq> RemoveUser u
-  \<longrightarrow> i_origin c \<triangleq> i
-  \<longrightarrow> (c_calls c \<triangleq> Call (DeleteKey (UserId u)) Undef)"
-
-definition inv3  where
-  "inv3 c_calls hb \<equiv> \<not>(\<exists>write delete u upd.
-    (\<exists>write_r. c_calls write \<triangleq> Call (NestedOp u upd) write_r)
+  "inv2 c_calls hb \<equiv> \<not>(\<exists>write delete u upd.
+    (cOp c_calls write \<triangleq> NestedOp u upd)
   \<and> is_update upd
-  \<and> (\<exists>delete_r. c_calls delete \<triangleq> Call (DeleteKey u) delete_r)
+  \<and> (cOp c_calls delete \<triangleq> DeleteKey u)
   \<and> (delete, write) \<in> hb
   )"
+
+definition inv3  where
+  "inv3 op i_origin c_calls \<equiv> \<forall>u i c.
+    op i \<triangleq> RemoveUser u
+  \<longrightarrow> i_origin c \<triangleq> i
+  \<longrightarrow> cOp c_calls c \<triangleq> DeleteKey (UserId u)"
 
 definition inv :: "(proc, operation, val) invContext \<Rightarrow> bool" where
   "inv ctxt \<equiv> 
     inv1 (invocOp ctxt) (invocRes ctxt) (invocation_happensBefore ctxt) 
-  \<and> inv2 (invocOp ctxt) (i_callOriginI ctxt) (calls ctxt)
-  \<and> inv3 (calls ctxt) (happensBefore ctxt)"
+  \<and> inv2 (calls ctxt) (happensBefore ctxt)
+  \<and> inv3 (invocOp ctxt) (i_callOriginI ctxt) (calls ctxt)"
+text_raw \<open>}%EndSnippet\<close>
 
-lemma show_inv[intro, case_names inv1 inv2 inv3]:
-  assumes "inv1 (invocOp ctxt) (invocRes ctxt) (invocation_happensBefore ctxt)" 
-    and "inv2 (invocOp ctxt) (i_callOriginI ctxt) (calls ctxt)" 
-    and "inv3 (calls ctxt) (happensBefore ctxt)"
-  shows "inv ctxt"
-  using assms  by (auto simp add: inv_def)
 
-lemma use_inv3:
-  assumes "inv3 c_calls hb"
-and "c_calls write \<triangleq> Call (NestedOp u upd) write_r"
-and "is_update upd"
-and "c_calls delete \<triangleq> Call (DeleteKey u) delete_r"
-and "(delete, write) \<in> hb"
-shows P
-  by (meson assms inv3_def)
 
-lemma use_inv3':
-  assumes "inv3 c_calls hb"
-and "c_calls write \<triangleq> Call (NestedOp u upd) write_r"
-and "is_update upd"
-and "c_calls delete \<triangleq> Call (DeleteKey u) delete_r"
-shows "(delete, write) \<notin> hb"
-  by (meson assms inv3_def)
+lemma use_inv2'':
+  assumes "inv2 c_calls hb"
+    and "cOp c_calls write \<triangleq> NestedOp u upd"
+    and "is_update upd"
+    and "cOp c_calls delete \<triangleq> DeleteKey u"
+  shows "(delete, write) \<notin> hb"
+  by (meson assms inv2_def)
+
+lemmas use_inv3 = inv3_def[unfolded atomize_eq, THEN iffD1, rule_format]
 
 definition userStruct :: "(userDataOp, val) crdtSpec" where
   "userStruct \<equiv> 
@@ -238,7 +229,7 @@ definition crdtSpec :: "(operation, val) crdtSpec" where
 
 
 definition userStruct' :: "('a, userDataOp, val) ccrdtSpec" where
-"userStruct' \<equiv> 
+  "userStruct' \<equiv> 
       struct_field' Name (register_spec' Undef) 
  .\<or>.. struct_field' Mail (register_spec' Undef)" 
 
@@ -305,9 +296,6 @@ qed
 lemma invariant_progr[simp]: "invariant progr = example_userbase.inv"
   by (auto simp add: progr_def)
 
-lemma if_distrib_eq: "(if c then x else y) = z \<longleftrightarrow> (if c then x = z else y = z)"
-  by (rule if_distrib)
-
 declare invContext.defs[simp]
 
 lemmas crdt_spec_defs = 
@@ -320,7 +308,7 @@ proof M_show_programCorrect
 
   case invariant_initial_state
   show "invariant_all' (initialState progr)"
-    by (simp add: example_userbase.inv_def initialState_def inv1_def inv2_def inv3_def invContextH2_happensBefore invContextH2_i_invocOp progr_def)
+    by (simp add: example_userbase.inv_def initialState_def inv1_def inv3_def inv2_def invContextH2_happensBefore invContextH2_i_invocOp progr_def)
 
   case (procedure_correct S i)
 
@@ -350,7 +338,7 @@ proof M_show_programCorrect
         case after_invocation
         show ?case 
           using show_P.invariant_pre RegisterUser
-          by (auto simp add:  inv_def inv1_def inv2_def inv3_def invContextH2_simps)
+          by (auto simp add:  inv_def inv1_def inv3_def invContextH2_simps)
 
       next
         case execution
@@ -392,76 +380,28 @@ proof M_show_programCorrect
             case (AtCommit v vn tx s_calls' s_happensBefore' s_callOrigin' s_txOrigin' s_knownIds' vis' s_invocOp' s_invocRes' c res ca resa PS')
 
 
-            have s_calls_mono: "s_calls' c \<triangleq> x" if "s_calls c \<triangleq> x" for c x
-              using AtCommit.ps_growing that
-              by (auto simp add: ps_growing_def proof_state_rel_calls dest!: state_monotonicGrowth_calls[where c=c and info=x])
-
-
-            have v_no_op1: "vn \<notin> uniqueIds op" if "s_calls' c \<triangleq> Call op r" for c op r
-            proof (rule new_unique_not_in_calls_def[THEN meta_eq_to_obj_eq, THEN iffD1, rule_format])
-              show " new_unique_not_in_calls s_calls' vn"
-                using AtCommit.uid_is_private'
-                by (meson AtCommit.uid_is_private'2 uid_is_private'_def)
-
-              show "s_calls' c \<triangleq> Call op r"
-                using that .
-            qed
-
-
-            hence v_no_op: "vn \<notin> uniqueIds op" if "s_calls c \<triangleq> Call op r" for c op r
-              using s_calls_mono that by blast
-
-
-            have v_no_delete1: False if "s_calls c \<triangleq> Call (DeleteKey v) Undef" for c
-              using v_no_op[OF that] AtCommit.uniqueIds_eq
-              by (auto simp add: uniqueIds_mapOp_def uniqueIds_val_def)
-
-
-            have v_no_delete2: "s_calls c \<noteq> Some (Call (DeleteKey v) Undef)" for c
-              using v_no_delete1 by blast
-
-
-            have v_no_op': "vn \<notin> uniqueIds op" if "s_calls' c \<triangleq> Call op r" for c op r
-            proof (rule new_unique_not_in_calls_def[THEN meta_eq_to_obj_eq, THEN iffD1, rule_format])
-              show " new_unique_not_in_calls s_calls' vn"
-                by (meson AtCommit.uid_is_private'2 uid_is_private'_def)
-
-              show "s_calls' c \<triangleq> Call op r"
-                using that .
-            qed
-
-
-            have v_no_delete1': False if "s_calls' c \<triangleq> Call (DeleteKey v) Undef" for c
-              using v_no_op'[OF that] ` uniqueIds v = {vn}`
-              by (auto simp add: uniqueIds_mapOp_def uniqueIds_val_def)
-
-            have v_no_delete2': "s_calls' c \<noteq> Some (Call (DeleteKey v) Undef)" for c
-              using v_no_delete1' by blast
-
-
-
-            from AtCommit
+            from AtCommit.inv
             show ?case
-            proof (auto simp add: inv_def, fuzzy_goal_cases inv1 inv2 inv3)
+            proof (auto simp add: inv_def AtCommit.PS'_eq, fuzzy_goal_cases inv1 inv2 inv3)
 
               case inv1
 
               from `inv1 (s_invocOp'(i \<mapsto> RegisterUser name mail)) (s_invocRes'(i := None))
                   (invocation_happensBeforeH (i_callOriginI_h s_callOrigin' s_txOrigin') s_happensBefore')`
               show ?case
+                using AtCommit.invocation_happensBeforeH_eq
                 by (auto simp add: inv1_def)
 
 
 
+
             next
-              case inv2
-              from `inv2 (s_invocOp'(i \<mapsto> RegisterUser name mail)) (i_callOriginI_h s_callOrigin' s_txOrigin') s_calls'`
-              show ?case
-                apply (auto simp add: inv2_def)
-                   apply (auto simp add: map_update_all_get i_callOriginI_h_simp)
-                by (auto simp add: i_callOriginI_h_update_to3 split: if_splits)
-            next 
               case inv3
+              from `inv3 (s_invocOp'(i \<mapsto> RegisterUser name mail)) (i_callOriginI_h s_callOrigin' s_txOrigin') s_calls'`
+              show ?case
+                by (auto simp add: inv3_def map_update_all_get i_callOriginI_h_simp i_callOriginI_h_update_to3 split: if_splits)
+            next 
+              case inv2
 
               from `uid_is_private' i s_calls' s_invocOp' s_invocRes' s_knownIds' vn`
               have "new_unique_not_in_calls s_calls' vn"
@@ -469,16 +409,12 @@ proof M_show_programCorrect
 
 
               text "Because v is a new unique id there can be no delete operation on that type:"
-              hence no_delete: "s_calls' delete \<noteq> Some (Call (DeleteKey v) delete_r)" for delete delete_r
-                using `uniqueIds v = {vn}` by (auto simp add: new_unique_not_in_calls_def uniqueIds_mapOp_def, force)
+              hence no_delete: "cOp s_calls' delete \<noteq> Some (DeleteKey v)" for delete
+                using `uniqueIds v = {vn}` by (auto simp add: new_unique_not_in_calls_def uniqueIds_mapOp_def cOp_Some_iff, force)
 
-                
-
-              from `inv3 s_calls' s_happensBefore'`
+              from `inv2 s_calls' s_happensBefore'`
               show ?case
-                by (auto simp add: no_delete inv3_def `c \<noteq> ca` updateHb_cases in_sequence_cons inv3(17) inv3(19) v_no_delete2')
-                
-
+                by (auto simp add: no_delete inv2_def  updateHb_cases in_sequence_cons  )
 
             qed
 
@@ -488,9 +424,7 @@ proof M_show_programCorrect
           next
             case (AtReturn v vn tx s_calls' s_happensBefore' s_callOrigin' s_txOrigin' s_knownIds' vis' s_invocOp' s_invocRes' c res ca resa)
             then show ?case
-              apply (auto simp add: inv_def)
-              apply (auto simp add: inv1_def )
-              by presburger
+              by (auto simp add: inv_def inv1_def split: if_splits)
           qed
 
         qed
@@ -504,7 +438,7 @@ proof M_show_programCorrect
         case after_invocation
         show ?case 
           using show_P.invariant_pre UpdateMail
-          by (auto simp add:  inv_def inv1_def inv2_def inv3_def invContextH2_simps)
+          by (auto simp add:  inv_def inv1_def inv3_def inv2_def invContextH2_simps)
 
       next
         case execution
@@ -542,123 +476,90 @@ proof M_show_programCorrect
             for  s_calls s_happensBefore s_callOrigin s_txOrigin s_knownIds s_invocOp s_invocRes
           proof (repliss_vcg_l, fuzzy_goal_cases "Exists_AtCommit" "Exists_AtReturn" "NotExists_AtCommit" "NotExists_AtReturn"  )
             case (Exists_AtCommit tx s_calls' s_happensBefore' s_callOrigin' s_txOrigin' s_knownIds' vis' s_invocOp' s_invocRes' c ca resa PS')
-            
+
             from Exists_AtCommit
             show ?case
             proof (auto simp add: inv_def, fuzzy_goal_cases inv1 inv2 inv3)
               case inv1
-              
+
               from `inv1 (s_invocOp'(i \<mapsto> UpdateMail user mail)) (s_invocRes'(i := None))
                (invocation_happensBeforeH (i_callOriginI_h s_callOrigin' s_txOrigin') s_happensBefore')`
               show ?case
                 by (auto simp add: inv1_def)
 
             next
-              case inv2
-              from `inv2 (s_invocOp'(i \<mapsto> UpdateMail user mail)) (i_callOriginI_h s_callOrigin' s_txOrigin') s_calls'`
+              case inv3
+              from `inv3 (s_invocOp'(i \<mapsto> UpdateMail user mail)) (i_callOriginI_h s_callOrigin' s_txOrigin') s_calls'`
               show ?case
-                using `c \<noteq> ca` by (auto simp add: inv2_def i_callOriginI_h_update_to3, meson)
+                by (auto simp add: inv3_def i_callOriginI_h_update_to3 split: if_splits)
 
             next
-              case inv3
+              case inv2
+
 
               from \<open>toplevel_spec crdtSpec' \<lparr>calls = s_calls', happensBefore = s_happensBefore'\<rparr> vis' (KeyExists (UserId user)) (Bool True)\<close>
-                obtain upd_c upd_op upd_r 
-                  where c0: "upd_c \<in> vis'"
-                    and c1: "is_update upd_op"
-                    and c2: "s_calls' upd_c \<triangleq> Call (NestedOp (UserId user) upd_op) upd_r"
-                    and c3: "\<forall>c'. c' \<in> vis' \<longrightarrow> (\<forall>r. s_calls' c' \<noteq> Some (Call (DeleteKey (UserId user)) r)) \<or> (c', upd_c) \<in> s_happensBefore'"
-                  apply (auto simp add: crdt_spec_defs)
-                  by (smt extract_op_eq inv3.less_eq subset_h1)
+
+              obtain upd_c upd_op
+                where a0: "upd_c \<in> vis'"
+                  and a1: "extract_op s_calls' upd_c = NestedOp (UserId user) upd_op"
+                  and a2: "is_update upd_op"
+                  and a3: "\<forall>d\<in>vis'. extract_op s_calls' d = DeleteKey (UserId user) \<longrightarrow> (d, upd_c) \<in> s_happensBefore'"
+                by (auto simp add: crdt_spec_defs)
 
 
-                show ?case
-                proof (auto simp add: inv3_def `c \<noteq> ca` `c \<noteq> ca`[symmetric])
+              from a1 
+              have a1': "cOp s_calls' upd_c \<triangleq> NestedOp (UserId user) upd_op"
+                by (metis (mono_tags, lifting) a0 cOp_Some extract_op_def in_dom inv2.less_eq option.sel)
 
-                  show "False"
-                    if d3: "is_update (Mail (Assign (String mail)))"
-                      and d0: "delete \<noteq> c"
-                      and d1: "delete \<noteq> ca"
-                      and d5: "(delete, ca) \<in> updateHb s_happensBefore' vis' [c, ca]"
-                      and d2: "s_calls' delete \<triangleq> Call (DeleteKey (UserId user)) delete_r"
-                    for  delete delete_r
-                  proof -
-                    from d5
-                    have "delete \<in> vis'"
-                      by (auto simp add: updateHb_cases in_sequence_cons `\<And>x y.  x = c \<or> x = ca \<Longrightarrow> (y, x) \<notin> s_happensBefore'` d0[symmetric])
+              from a3 
+              have a3': "\<forall>d\<in>vis'. cOp s_calls' d \<triangleq> DeleteKey (UserId user) \<longrightarrow> (d, upd_c) \<in> s_happensBefore'"
+                by (meson extract_op_eq' inv2.less_eq subset_iff)
 
 
-                    from c3[rule_format, OF `delete \<in> vis'`]
-                    have "(delete, upd_c) \<in> s_happensBefore'"
-                      by (auto simp add: d2)
+              text \<open>There can be no delete:\<close>
 
-                    text "This violates invariant 3"
-                    with `inv3 s_calls' s_happensBefore'` c2 c1 d2
-                    show False
-                      apply (auto simp add: inv3_def)
-                      by blast
-                  qed
+              have noDelete: "delete \<notin> vis'" if "cOp s_calls' delete \<triangleq> DeleteKey (UserId user)" for delete
+                using use_inv2''[OF \<open>inv2 s_calls' s_happensBefore'\<close> a1' a2 that] a3' that by blast
 
-                  show "False"
-                    if d0: "write \<noteq> c"
-                      and d1: "write \<noteq> ca"
-                      and d2: "delete \<noteq> c"
-                      and d3: "delete \<noteq> ca"
-                      and d4: "is_update upd"
-                      and d5: "s_calls' write \<triangleq> Call (NestedOp u upd) write_r"
-                      and d6: "(delete, write) \<in> updateHb s_happensBefore' vis' [c, ca]"
-                      and d7: "s_calls' delete \<triangleq> Call (DeleteKey u) delete_r"
-                    for "write" delete u upd write_r delete_r
-                  proof - text "From old invariant ... "
-                    from d6
-                    have "(delete, write) \<in> s_happensBefore'"
-                      by (metis d0 d1  insert_iff list.set(1) list.simps(15) singletonD updateHb_simp2)
+              text \<open>With this we can show that inv2 is maintained:\<close>
 
+              show ?case
+                using noDelete inv2.not_member3 use_inv2''[OF inv2.inv2]
+                by (auto simp add: inv2_def `c \<noteq> ca` `c \<noteq> ca`[symmetric] updateHb_cons)
 
-                    with `inv3 s_calls' s_happensBefore'` d4 d5 d7 
-                    show False
-                      by (auto simp add: inv3_def, blast)
-
-                  qed
-                qed
-              qed
-
-            next
-              case (Exists_AtReturn tx s_calls' s_happensBefore' s_callOrigin' s_txOrigin' s_knownIds' vis' s_invocOp' s_invocRes' c ca resa)
-              then show ?case
-                by (auto simp add: inv_def inv1_def, presburger) 
-            next
-              case (NotExists_AtCommit tx s_calls' s_happensBefore' s_callOrigin' s_txOrigin' s_knownIds' vis' s_invocOp' s_invocRes' c res PS')
-
-              
-
-
-              
-              show ?case 
-                using NotExists_AtCommit.invocation_happensBeforeH_eq
-                using NotExists_AtCommit.inv
-                by (auto simp add: inv_def inv1_def inv2_def inv3_def 
-                      i_callOriginI_h_update_to3 map_update_all_get updateHb_single NotExists_AtCommit.PS'_eq, meson)
-
-
-
-            next
-              case (NotExists_AtReturn tx s_calls' s_happensBefore' s_callOrigin' s_txOrigin' s_knownIds' vis' s_invocOp' s_invocRes' c res)
-              then show ?case 
-                by (auto simp add: inv_def inv1_def, presburger) 
             qed
+
+          next
+            case (Exists_AtReturn tx s_calls' s_happensBefore' s_callOrigin' s_txOrigin' s_knownIds' vis' s_invocOp' s_invocRes' c ca resa)
+            then show ?case
+              by (auto simp add: inv_def inv1_def, presburger) 
+          next
+            case (NotExists_AtCommit tx s_calls' s_happensBefore' s_callOrigin' s_txOrigin' s_knownIds' vis' s_invocOp' s_invocRes' c res PS')
+
+
+            show ?case 
+              using NotExists_AtCommit.invocation_happensBeforeH_eq
+              using NotExists_AtCommit.inv
+              by (auto simp add: inv_def inv1_def inv3_def inv2_def 
+                  i_callOriginI_h_update_to3 map_update_all_get updateHb_single NotExists_AtCommit.PS'_eq, meson)
+
+          next
+            case (NotExists_AtReturn tx s_calls' s_happensBefore' s_callOrigin' s_txOrigin' s_knownIds' vis' s_invocOp' s_invocRes' c res)
+            then show ?case 
+              by (auto simp add: inv_def inv1_def, presburger) 
           qed
         qed
+      qed
 
     next
       case (RemoveUser user)
-      
+
       show "procedureCorrect S i"
       proof M_show_procedureCorrect
         case after_invocation
         show ?case 
           using show_P.invariant_pre RemoveUser
-          apply (auto simp add:  inv_def inv1_def inv2_def inv3_def invContextH2_simps)
+          apply (auto simp add:  inv_def inv1_def inv3_def inv2_def invContextH2_simps)
           using new_invocation_cannot_happen_before show_P.i_fresh show_P.wf_pre apply blast
           using i_callOriginI_notI1 show_P.i_fresh show_P.wf_pre by blast
 
@@ -701,51 +602,47 @@ proof M_show_programCorrect
           proof (repliss_vcg_l, fuzzy_goal_cases "Exists_AtCommit" "Exists_AtReturn" )
             case (Exists_AtCommit tx s_calls' s_happensBefore' s_callOrigin' s_txOrigin' s_knownIds' vis' s_invocOp' s_invocRes' c res PS')
 
-            from \<open>toplevel_spec crdtSpec' \<lparr>calls = s_calls', happensBefore = s_happensBefore'\<rparr> vis' (DeleteKey (UserId user)) res\<close>
-            have [simp]: "res= Undef"
-              by (auto simp add: crdt_spec_defs)
 
-            from Exists_AtCommit
+            from Exists_AtCommit.inv Exists_AtCommit.invocation_happensBeforeH_eq
             show ?case
-            proof (auto simp add: inv_def, fuzzy_goal_cases inv1 inv2 inv3)
+            proof (auto simp add: inv_def Exists_AtCommit.PS'_eq, fuzzy_goal_cases inv1 inv2 inv3)
               case inv1
               from `inv1 (s_invocOp'(i \<mapsto> RemoveUser user)) (s_invocRes'(i := None))
                    (invocation_happensBeforeH (i_callOriginI_h s_callOrigin' s_txOrigin') s_happensBefore')`
               show ?case
                 by (auto simp add: inv1_def)
 
-              
-            next
-              case inv2
-              from `inv2 (s_invocOp'(i \<mapsto> RemoveUser user)) (i_callOriginI_h s_callOrigin' s_txOrigin') s_calls'`
-              show ?case 
-                apply (auto simp add: inv2_def i_callOriginI_h_update_to3   `\<And>c. s_callOrigin' c \<noteq> Some tx`)
-                using inv2(2) by force+
-
             next
               case inv3
-              from `inv3 s_calls' s_happensBefore'`
+              from `inv3 (s_invocOp'(i \<mapsto> RemoveUser user)) (i_callOriginI_h s_callOrigin' s_txOrigin') s_calls'`
+              show ?case 
+                by (auto simp add: inv3_def i_callOriginI_h_update_to3   `\<And>c. s_callOrigin' c \<noteq> Some tx` split: if_splits)
+
+            next
+              case inv2
+              from `inv2 s_calls' s_happensBefore'`
               show ?case
-                by (auto simp add: inv3_def updateHb_cases  in_sequence_cons  inv3)
+                using Exists_AtCommit.not_member2
+                by (auto simp add: inv2_def updateHb_cases  in_sequence_cons  inv2)
+
             qed
 
           next
-             case (Exists_AtReturn tx s_calls' s_happensBefore' s_callOrigin' s_txOrigin' s_knownIds' vis' s_invocOp' s_invocRes' c res)
+            case (Exists_AtReturn tx s_calls' s_happensBefore' s_callOrigin' s_txOrigin' s_knownIds' vis' s_invocOp' s_invocRes' c res)
             then show ?case
-              apply (auto simp add: inv_def inv1_def)
-              by presburger+
+              by (auto simp add: inv_def inv1_def split: if_splits)
           qed
         qed
       qed
     next
       case (GetUser user)
-  
+
       show "procedureCorrect S i"
       proof M_show_procedureCorrect
         case after_invocation
         show ?case 
           using show_P.invariant_pre GetUser
-          by (auto simp add:  inv_def inv1_def inv2_def inv3_def invContextH2_simps  new_invocation_cannot_happen_after)
+          by (auto simp add:  inv_def inv1_def inv3_def inv2_def invContextH2_simps  new_invocation_cannot_happen_after)
 
 
       next
@@ -783,54 +680,75 @@ proof M_show_programCorrect
             for  s_calls s_happensBefore s_callOrigin s_txOrigin s_knownIds s_invocOp s_invocRes
           proof (repliss_vcg_l, fuzzy_goal_cases "Exists_AtCommit" "Exists_AtReturn" "NotExists_AtCommit" "NotExists_AtReturn"  )
             case (Exists_AtCommit tx s_calls' s_happensBefore' s_callOrigin' s_txOrigin' s_knownIds' vis' s_invocOp' s_invocRes' c ca resa cb res PS')
-            then show ?case
-            proof (auto simp add: inv_def, fuzzy_goal_cases inv1 inv2 inv3)
+
+            from Exists_AtCommit.inv
+            show ?case
+            proof (auto simp add: inv_def Exists_AtCommit.PS'_eq, fuzzy_goal_cases inv1 inv2 inv3)
               case (inv1)
               then show ?case
+                using Exists_AtCommit.invocation_happensBeforeH_eq
                 by (auto simp add: inv1_def)
-            next
-              case (inv2)
-              then show ?case 
-                apply (auto simp add: inv2_def)
-                apply (metis i_callOriginI_h_update_to2 list.set_intros(1) map_update_all_get option.inject)
-                apply (metis (no_types, lifting) i_callOriginI_h_update_to2 insertCI list.simps(15) map_update_all_get option.inject)
-                 apply (metis (no_types, lifting) i_callOriginI_h_update_to2 insertCI list.simps(15) map_update_all_get option.inject)
-                by (smt i_callOriginI_h_def i_callOriginI_h_update_to2 map_update_all_get option.inject)
+
+
             next
               case (inv3)
               then show ?case 
-                by (auto simp add: inv3_def i_callOriginI_h_update_to3 updateHb_cases in_sequence_cons is_update_userDataOp_def)
+                using Exists_AtCommit.not_ca_eq Exists_AtCommit.not_c_eq Exists_AtCommit.not_c_eq2
+                by (auto simp add: inv3_def i_callOriginI_h_update_to3 split: if_splits)
+            next
+              case (inv2)
+              then show ?case 
+                by (auto simp add: inv2_def i_callOriginI_h_update_to3 updateHb_cases in_sequence_cons is_update_userDataOp_def)
             qed  
-              
+
           next
             case (Exists_AtReturn tx s_calls' s_happensBefore' s_callOrigin' s_txOrigin' s_knownIds' vis' s_invocOp' s_invocRes' c ca resa cb res)
-            then show ?case
-            proof (auto simp add: inv_def, fuzzy_goal_cases inv1 )
+
+            find_theorems name: "Exists_AtReturn." 
+
+            from Exists_AtReturn.inv
+            show ?case
+            proof (auto simp add: inv_def, fuzzy_goal_cases inv1 inv2 inv3)
               case (inv1)
+
 
               text "From the query result, we get an update that is not affected by a remove."
 
               from \<open>toplevel_spec crdtSpec' \<lparr>calls = s_calls', happensBefore = s_happensBefore'\<rparr> vis' (KeyExists (UserId user)) (Bool True)\<close>
-              obtain upd_c upd_op upd_r
+              obtain upd_c upd_op
                 where upd_c0: "upd_c \<in> vis'"
-                  and upd_c1: "is_update upd_op"
-                  and upd_c2: "s_calls' upd_c \<triangleq> Call (NestedOp (UserId user) upd_op) upd_r"
-                  and upd_c3: "\<forall>c'. c' \<in> vis' \<longrightarrow> (\<forall>r. s_calls' c' \<noteq> Some (Call (DeleteKey (UserId user)) r)) \<or> (c', upd_c) \<in> s_happensBefore'"
-                apply (auto simp add: crdt_spec_defs  split: if_splits)
-                by (smt extract_op_eq in_mono inv1.less_eq)
+                  and upd_c1: "extract_op s_calls' upd_c = NestedOp (UserId user) upd_op"
+                  and upd_c2: "is_update upd_op"
+                  and upd_c3: "\<forall>d\<in>vis'. extract_op s_calls' d = DeleteKey (UserId user) \<longrightarrow> (d, upd_c) \<in> s_happensBefore'"
+                by (auto simp add: crdt_spec_defs  split: if_splits)
+
+              from upd_c1
+              have upd_c1': "cOp s_calls' upd_c \<triangleq> NestedOp (UserId user) upd_op"
+                by (metis Exists_AtReturn.less_eq extract_op_eq' in_mono upd_c0)
 
 
+              from upd_c3
+              have upd_c3': "(d, upd_c) \<in> s_happensBefore'"
+                if "cOp s_calls' d \<triangleq> DeleteKey (UserId user)"
+                  and "d \<in> vis'"
+                for d
+                using that
+                by (meson extract_op_eq' Exists_AtReturn.less_eq subset_iff)
 
-
-              text "No calls means we do not have any invocation happened before"
+              text "No calls means we do not have any invocation happened before in the pre-state."
               have no_hb: "(r, i) \<notin> invocation_happensBeforeH (i_callOriginI_h s_callOrigin' s_txOrigin') s_happensBefore'" for r
-                using inv1(5) by (auto simp add: invocation_happensBeforeH_def i_callOriginI_h_def split: option.splits)
+                using Exists_AtReturn.not_s_txOrigin'_eq by (auto simp add: invocation_happensBeforeH_def i_callOriginI_h_def split: option.splits)
+
 
               have [simp]: "s_txOrigin'(tx := None) = s_txOrigin'"
-                  by (simp add: fun_upd_idem_iff inv1.s_txOrigin'___eq)
-              
+                by (simp add: fun_upd_idem_iff Exists_AtReturn.s_txOrigin'_eq)
+
+
               show ?case
-              proof (auto simp add: inv1_def no_hb)
+              proof (auto simp add: inv1_def no_hb Exists_AtReturn.invocation_happensBeforeH_eq)
+
+
+
 
                 show "\<exists>c''. i_callOriginI_h s_callOrigin' s_txOrigin' c'' \<triangleq> r \<and> c'' \<notin> vis'"
                   if c0: "r \<noteq> i"
@@ -838,8 +756,29 @@ proof M_show_programCorrect
                     and c3: "i_callOriginI_h s_callOrigin' s_txOrigin' c' \<triangleq> r"
                     and c4: "c' \<in> vis'"
                   for  r c'
-                  using use_inv3'[OF `inv3 s_calls' s_happensBefore'`]
-                  by (smt c1 c3 fun_upd_triv inv1.inv2 inv1.s_invocOp'___eq inv2_def upd_c1 upd_c2 upd_c3)
+                proof -
+
+                  from c1 c0
+                  have c1': \<open>(s_invocOp'(i \<mapsto> GetUser user)) r \<triangleq> RemoveUser user\<close> by simp
+
+
+                  text \<open>use inv3 to get the delete operation\<close>
+
+                  from use_inv3[OF inv1.inv3 c1' c3]
+                  have "cOp s_calls' c' \<triangleq> DeleteKey (UserId user)" .
+
+
+                  text \<open>The delete must be before upd_c by the CRDT spec (otherwise entry would not exist)\<close>
+
+                  from upd_c3'[OF \<open>cOp s_calls' c' \<triangleq> DeleteKey (UserId user)\<close> c4]
+                  have "(c', upd_c) \<in> s_happensBefore'" .
+
+                  from use_inv2''[OF inv1.inv2 upd_c1' upd_c2 \<open>cOp s_calls' c' \<triangleq> DeleteKey (UserId user)\<close>]
+                  have \<open>(c', upd_c) \<notin> s_happensBefore'\<close>  .
+
+                  with \<open>(c', upd_c) \<in> s_happensBefore'\<close>
+                  show ?thesis by blast
+                qed
 
                 show "g_res = NotFound"
                   if c0: "r \<noteq> i"
@@ -857,11 +796,21 @@ proof M_show_programCorrect
 
 
               qed
+
+            next
+              case inv2
+              thus ?case
+                by (auto simp add: inv2_def Exists_AtReturn is_update_userDataOp_def updateHb_simp2)
+            next
+              case inv3
+              thus ?case
+                by (auto simp add: inv3_def Exists_AtReturn i_callOriginI_h_update_to3 split: if_splits)
+
             qed
           next
             case (NotExists_AtCommit tx s_calls' s_happensBefore' s_callOrigin' s_txOrigin' s_knownIds' vis' s_invocOp' s_invocRes' c res)
             then show ?case 
-              by (auto simp add: inv_def inv1_def inv2_def inv3_def i_callOriginI_h_update_to3 map_update_all_get updateHb_cases in_sequence_cons split: if_splits, meson)
+              by (auto simp add: inv_def inv1_def inv3_def inv2_def i_callOriginI_h_update_to3 map_update_all_get updateHb_cases in_sequence_cons split: if_splits, meson)
 
           next
             case (NotExists_AtReturn tx s_calls' s_happensBefore' s_callOrigin' s_txOrigin' s_knownIds' vis' s_invocOp' s_invocRes' c res)
@@ -873,5 +822,6 @@ proof M_show_programCorrect
     qed
   qed
 qed
+
 
 end
